Use Coq features to shorten things

mechanization/theories/PtsSignature.v
@@ -1,10 +1,10 @@
-From Coq Require Import Relation_Definitions RelationClasses.
+From Coq Require Import Orders Relation_Definitions RelationClasses.
 
 From Equations Require Import Equations.
 
 Record PtsSig : Type :=
-  mkPtsSig{
-      St : Set;
+  mkPtsSig {
+      St :> Set;
       Ax : St -> St -> Set;
       Ru : St -> St -> St -> Set;
     }.
@@ -12,12 +12,12 @@ Record PtsSig : Type :=
 (* It would be nicer to have this in Prop, but Rocq complains *)
 Record PredicativeSig (P : PtsSig) : Type :=
   mkPredicativeSig {
-      pred_rel : relation (St P);
-      pred_irrel : forall {s1 s2 : St P} (lt lt' : pred_rel s1 s2), lt = lt';
-      ord_rel : order (St P) (fun s1 s2 => pred_rel s1 s2 \/ s1 = s2);
+      pred_rel : relation P;
+      pred_irrel : forall {s1 s2 : P} (lt lt' : pred_rel s1 s2), lt = lt';
+      ord_rel : StrictOrder pred_rel;
       wf_rel : well_founded pred_rel;
-      ord_ax : forall {s1 s2 : St P}, Ax P s1 s2 -> pred_rel s1 s2;
-      ord_ru : forall {s1 s2 s3 : St P}, Ru P s1 s2 s3 -> (pred_rel s1 s3 \/ s1 = s3) /\ (pred_rel s2 s3 \/ s2 = s3);
+      ord_ax : forall {s1 s2 : P}, Ax P s1 s2 -> pred_rel s1 s2;
+      ord_ru : forall {s1 s2 s3 : P}, Ru P s1 s2 s3 -> (pred_rel s1 s3 \/ s1 = s3) /\ (pred_rel s2 s3 \/ s2 = s3);
     }.
 Arguments pred_rel {_}.
 Arguments pred_irrel {_} _ {_ _}.
@@ -25,3 +25,40 @@ Arguments ord_rel {_}.
 Arguments wf_rel {_}.
 Arguments ord_ax {_} _ {_ _}.
 Arguments ord_ru {_} _ {_ _ _}.
+
+Section OrderProperties.
+  Context {P : PtsSig} (pred_P : PredicativeSig P).
+
+  Instance pred_rel_StrictOrder : StrictOrder (pred_rel pred_P) := ord_rel pred_P.
+  Opaque pred_rel_StrictOrder.
+
+  Instance pred_rel_WellFounded : WellFounded (pred_rel pred_P) := wf_rel pred_P.
+  Opaque pred_rel_WellFounded.
+
+  Instance pred_rel_Asymmetric : Asymmetric (pred_rel pred_P).
+  Proof using.
+    typeclasses eauto.
+  Qed.
+
+  Let clos_refl_rel := fun s1 s2 => pred_rel pred_P s1 s2 \/ s1 = s2.
+
+  Instance clos_refl_rel_Reflexive : Reflexive clos_refl_rel.
+  Proof using.
+    solve [do 2 constructor].
+  Qed.
+
+  Instance clos_refl_rel_Transitive : Transitive clos_refl_rel.
+  Proof using.
+    intros ? * [] []; subst; try solve [do 2 constructor]; constructor; eauto.
+    etransitivity; eauto.
+  Qed.
+
+  Lemma ord_clos_refl_rel : order P clos_refl_rel.
+    constructor.
+    - intro. reflexivity.
+    - intros ? **.
+      etransitivity; eassumption.
+    - intros ? * [] Hyx; inversion_clear Hyx; subst; eauto.
+      exfalso. eapply pred_rel_Asymmetric; eassumption.
+  Qed.
+End OrderProperties.
